theories/Syntax/Messages.v
@@ -91,6 +91,9 @@ Module Type MessagesOn
         | there msg => there <$> occurs_check (ctx.in_succ xIn) msg
         end.
 
+    #[export] Instance erase_closemessage `{Erase M ME} : Erase (CloseMessage M) ME | 2 :=
+      fun {Σ} m => match m with there msg => erase msg end.
+
     (* #[export] Instance genoccurscheck_closemessage `{SubstSU WeakensTo M} {ocM : GenOccursCheck M} : GenOccursCheck (sSUT := substSU_closemessage) (CloseMessage M) | 2 := *)
     (*   fun {Σ} m => *)
     (*     match m with *)
@@ -100,12 +103,12 @@ Module Type MessagesOn
     (*     end. *)
 
     Inductive AMessage (Σ : LCtx) : Type :=
-    | mk {M} {subM : Subst M} {wkM : SubstSU WeakensTo M} {wkM : SubstSULaws WeakensTo M} {subLM : SubstLaws M} {occM: OccursCheck M} (msg : M Σ).
-    #[global] Arguments mk {_ _ _ _ _ _ _} msg.
+    | mk {M} {subM : Subst M} {wkM : SubstSU WeakensTo M} {wkML : SubstSULaws WeakensTo M} {subLM : SubstLaws M} {occM: OccursCheck M} {ME : Type} {eM : Erase M ME} (msg : M Σ).
+    #[global] Arguments mk {_ _ _ _ _ _ _ _ _} msg.
 
     Definition empty {Σ} : AMessage Σ := mk (M := Unit) tt.
 
-    Fixpoint closeAux {Σ ΣΔ} {M} {suM : SubstSU WeakensTo M} {suLM : SubstSULaws WeakensTo M} {subM : Subst M} {subLM : SubstLaws M} {occM: OccursCheck M} {struct ΣΔ} : M (Σ ▻▻ ΣΔ) -> AMessage Σ :=
+    Fixpoint closeAux {Σ ΣΔ} {M} {suM : SubstSU WeakensTo M} {suLM : SubstSULaws WeakensTo M} {subM : Subst M} {subLM : SubstLaws M} {occM: OccursCheck M} {ME : Type} {eM : Erase M ME} {struct ΣΔ} : M (Σ ▻▻ ΣΔ) -> AMessage Σ :=
       match ΣΔ with
       | []      => fun msg => mk msg
       | ΣΔ  ▻ b => fun msg => closeAux (suM := substSU_closemessage) (subM := subst_closemessage) (there msg)
@@ -148,37 +151,20 @@ Module Type MessagesOn
         | mk msg    => mk <$> occurs_check xIn msg
         end.
 
-      (* During unquantify, we want to stop treating debug messages as substitutable,
-         because messages often mention many variables that play no other role
-         and they should be unquantified away.
+    Inductive EAMessage : Type :=
+    | MkEAMessage : forall {M : Type}, M -> EAMessage
+    .
 
-         More generally, we do this during every gen_occurs_check.
+    #[export] Instance erase_amessage : Erase AMessage EAMessage :=
+      fun {Σ} '(amsg.mk m) => MkEAMessage (erase m).
 
-         This has the downside that boxed messages will no longer be subject to
-         substitution, but as long as unquantify and other clients of gen_occurs_check
-         are executed after other
-         simplification passes have run, no information should get lost.
-       *)
-      Definition BoxMessage (M : LCtx -> Type) : LCtx -> Type := Const {Σ' : LCtx & M Σ'}.
-      Definition boxMsg' {M Σ Σ'}  : M Σ -> BoxMessage M Σ' := existT _.
-      Definition boxMsg {Σ Σ'}  (msg : AMessage Σ) : AMessage Σ' :=
-        match msg with
-          amsg.mk msg => amsg.mk (boxMsg' msg)
-        end.
+    Definition boxMsg {Σ Σ'}  (msg : AMessage Σ) : AMessage Σ' :=
+      match msg with
+        amsg.mk msg => amsg.mk (M := Const _) (erase msg)
+      end.
 
     #[export] Instance genoccurscheck_amessage : GenOccursCheck AMessage :=
-      fix oc {Σ} m {struct m} :=
-        match m with
-        | mk msg    => weakenInit (amsg.mk (boxMsg' msg))
-        end.
-
-    (* #[export] Instance genoccurschecklaws_amessage : GenOccursCheckLaws AMessage. *)
-    (* Proof. *)
-    (*   constructor. *)
-    (*   destruct t. *)
-    (*   (* TODO: add laws instance for contained messages *) *)
-    (*   admit. *)
-    (* Admitted. *)
+      fun {_} m => weakenInit (boxMsg m).
 
     #[export] Instance instprop_amessage : InstProp AMessage :=
       fun _ _ _ => True.
